wip

crypto/bignum/Hacl.Bignum.Parameters.fsti
@@ -1,5 +1,6 @@
 module Hacl.Bignum.Parameters
 
+open FStar.Mul
 open FStar.HyperStack
 open FStar.Buffer
 
@@ -7,18 +8,12 @@ open FStar.Buffer
 val prime: pos
 
 (** Size of a word on the platform (32 or 64bits) **)
-val word_size: ws:pos{ws = 32 \/ ws = 64}
+val word_size: ws:pos
 
 (** Concrete platform word with side-channel protection **)
-(* inline_for_extraction let limb = if word_size = 32 then Hacl.UInt32.t else Hacl.UInt64.t *)
-(* inline_for_extraction let wide = if word_size = 32 then Hacl.UInt64.t else Hacl.UInt128.t *)
 inline_for_extraction val limb: Type0
 inline_for_extraction val wide: Type0
 inline_for_extraction let ctr  = FStar.UInt32.t
-
-
-val v: limb -> GTot nat
-val w: wide -> GTot nat
 
 
 (** Number of limbs of a bigint **)
@@ -30,18 +25,81 @@ type felem_wide = b:buffer wide{length b = len}
 
 
 (** Associates a weight in bits to each limb of the bigint *)
-(* val template: idx:nat{idx < len} -> Tot pos *)
-(* val ctemplate: *)
-(*   idx:FStar.UInt32.t{FStar.UInt32.v idx < len} -> *)
-(*   Tot (x:FStar.UInt32.t{template (FStar.UInt32.v idx) = FStar.UInt32.v x}) *)
 val limb_size: pos
 inline_for_extraction val climb_size: l:FStar.UInt32.t{limb_size = FStar.UInt32.v l}
 
-(** Predicate associated to 'workable' bigintegers, restored after each bigint computation **)
-val reduced_after_mul: h:mem -> b:felem -> GTot Type0
-val reduced_before_mul_l: h:mem -> b:felem -> GTot Type0
-val reduced_before_mul_r: h:mem -> b:felem -> GTot Type0
-val reduced_wide: h:mem -> b:felem_wide -> GTot Type0
+val lemma_prime_limb_size: unit -> Lemma (pow2 (len * limb_size) > prime)
 
-(** Predicate associated to 'workable' bigintegers, restored after each bigint computation **)
-val reducible: h:mem -> b:felem -> GTot Type0
+(* Limb operators *)
+inline_for_extraction let limb_n = word_size
+inline_for_extraction val v: limb -> GTot (FStar.UInt.uint_t limb_n)
+
+inline_for_extraction val limb_zero: x:limb{v x = 0}
+inline_for_extraction val limb_one: x:limb{v x = 1}
+
+(* Addition primitives *)
+inline_for_extraction val limb_add: a:limb -> b:limb{UInt.size (v a + v b) limb_n} -> Tot (c:limb{v a + v b = v c})
+inline_for_extraction val limb_add_mod: a:limb -> b:limb -> Tot (c:limb{(v a + v b) % pow2 limb_n = v c})
+(* Subtraction primitives *)
+inline_for_extraction val limb_sub: a:limb -> b:limb{UInt.size (v a - v b) limb_n} -> Tot (c:limb{v a - v b = v c})
+inline_for_extraction val limb_sub_mod: a:limb -> b:limb -> Tot (c:limb{(v a - v b) % pow2 limb_n = v c})
+(* Multiplication primitives *)
+inline_for_extraction val limb_mul: a:limb -> b:limb{UInt.size (v a * v b) limb_n} -> Tot (c:limb{v a * v b = v c})
+inline_for_extraction val limb_mul_mod: a:limb -> b:limb -> Tot (c:limb{(v a * v b) % pow2 limb_n = v c})
+
+(* Bitwise operators *)
+inline_for_extraction val limb_logand: limb -> limb -> Tot limb
+inline_for_extraction val limb_logxor: limb -> limb -> Tot limb
+inline_for_extraction val limb_logor: limb -> limb -> Tot limb
+inline_for_extraction val limb_lognot: limb -> Tot limb
+
+(* Shift operators *)
+inline_for_extraction val limb_shift_right: a:limb -> s:FStar.UInt32.t -> Tot (c:limb{FStar.UInt32.v s < limb_n ==> v c = (v a / (pow2 (FStar.UInt32.v s)))})
+inline_for_extraction val limb_shift_left: a:limb -> s:FStar.UInt32.t -> Tot (c:limb{FStar.UInt32.v s < limb_n ==> v c = ((v a * pow2 (FStar.UInt32.v s)) % pow2 limb_n)})
+
+inline_for_extraction val limb_eq_mask: a:limb -> b:limb -> Tot (c:limb{(v a = v b ==> v c = pow2 limb_n - 1) /\ (v a <> v b ==> v c = 0)})
+inline_for_extraction val limb_gte_mask: a:limb -> b:limb -> Tot (c:limb{(v a >= v b ==> v c = pow2 limb_n - 1) /\ (v a < v b ==> v c = 0)})
+inline_for_extraction val limb_gt_mask: a:limb -> b:limb -> Tot (c:limb{(v a > v b ==> v c = pow2 limb_n - 1) /\ (v a <= v b ==> v c = 0)})
+inline_for_extraction val limb_lt_mask: a:limb -> b:limb -> Tot (c:limb{(v a < v b ==> v c = pow2 limb_n - 1) /\ (v a >= v b ==> v c = 0)})
+inline_for_extraction val limb_lte_mask: a:limb -> b:limb -> Tot (c:limb{(v a <= v b ==> v c = pow2 limb_n - 1) /\ (v a > v b ==> v c = 0)})
+
+inline_for_extraction val limb_to_byte: x:limb -> Tot (y:Hacl.UInt8.t{Hacl.UInt8.v y = v x % pow2 8})
+inline_for_extraction val byte_to_limb: x:Hacl.UInt8.t -> Tot (y:limb{Hacl.UInt8.v x = v y})
+
+
+(* Wide limb operators *)
+inline_for_extraction let wide_n = 2 * word_size
+
+inline_for_extraction val w: wide -> GTot (FStar.UInt.uint_t wide_n)
+
+inline_for_extraction val wide_zero: x:wide{w x = 0}
+inline_for_extraction val wide_one: x:wide{w x = 1}
+
+(* Addition primitives *)
+inline_for_extraction val wide_add: a:wide -> b:wide{UInt.size (w a + w b) wide_n} -> Tot (c:wide{w a + w b = w c})
+inline_for_extraction val wide_add_mod: a:wide -> b:wide -> Tot (c:wide{(w a + w b) % pow2 wide_n = w c})
+(* Subtraction primitives *)
+inline_for_extraction val wide_sub: a:wide -> b:wide{UInt.size (w a - w b) wide_n} -> Tot (c:wide{w a - w b = w c})
+inline_for_extraction val wide_sub_mod: a:wide -> b:wide -> Tot (c:wide{(w a - w b) % pow2 wide_n = w c})
+(* Bitwise operators *)
+inline_for_extraction val wide_logand: wide -> wide -> Tot wide
+inline_for_extraction val wide_logxor: wide -> wide -> Tot wide
+inline_for_extraction val wide_logor: wide -> wide -> Tot wide
+inline_for_extraction val wide_lognot: wide -> Tot wide
+
+(* Shift operators *)
+inline_for_extraction val wide_shift_right: a:wide -> s:FStar.UInt32.t -> Tot (c:wide{FStar.UInt32.v s < wide_n ==> w c = (w a / (pow2 (FStar.UInt32.v s)))})
+inline_for_extraction val wide_shift_left: a:wide -> s:FStar.UInt32.t -> Tot (c:wide{FStar.UInt32.v s < wide_n ==> w c = ((w a * pow2 (FStar.UInt32.v s)) % pow2 wide_n)})
+
+inline_for_extraction val wide_eq_mask: a:wide -> b:wide -> Tot (c:wide{(w a = w b ==> w c = pow2 wide_n - 1) /\ (w a <> w b ==> w c = 0)})
+inline_for_extraction val wide_gte_mask: a:wide -> b:wide -> Tot (c:wide{(w a >= w b ==> w c = pow2 wide_n - 1) /\ (w a < w b ==> w c = 0)})
+inline_for_extraction val wide_gt_mask: a:wide -> b:wide -> Tot (c:wide{(w a > w b ==> w c = pow2 wide_n - 1) /\ (w a <= w b ==> w c = 0)})
+inline_for_extraction val wide_lt_mask: a:wide -> b:wide -> Tot (c:wide{(w a < w b ==> w c = pow2 wide_n - 1) /\ (w a >= w b ==> w c = 0)})
+inline_for_extraction val wide_lte_mask: a:wide -> b:wide -> Tot (c:wide{(w a <= w b ==> w c = pow2 wide_n - 1) /\ (w a > w b ==> w c = 0)})
+
+inline_for_extraction val mul_wide: a:limb -> b:limb -> Tot (c:wide{w c = v a * v b})
+
+inline_for_extraction let op_Star_Hat = mul_wide
+
+inline_for_extraction val limb_to_wide: x:limb -> Tot (y:wide{w y = v x})
+inline_for_extraction val wide_to_limb: x:wide -> Tot (y:limb{v y = w x % pow2 limb_n})
