crypto/bignum/x25519/Hacl.Bignum.Parameters.fst
@@ -2,6 +2,7 @@ module Hacl.Bignum.Parameters
 
 open FStar.HyperStack
 open FStar.Buffer
+open Hacl.Cast
 
 let prime =
   assert_norm (pow2 255 > 19);
@@ -12,35 +13,108 @@ let word_size = 64
 inline_for_extraction let limb = Hacl.UInt64.t
 inline_for_extraction let wide = Hacl.UInt128.t
 
-let v x = Hacl.UInt64.v x
-let w x = Hacl.UInt128.v x
-
 let len = 5
 inline_for_extraction let clen = 5ul
 
 let limb_size = 51
 inline_for_extraction let climb_size = 51ul
 
-let reduced_after_mul h b =
-  let _ = 0 in
-  live h b /\ v (get h b 0) < pow2 52 /\ v (get h b 1) < pow2 52 /\ v (get h b 2) < pow2 52
-  /\ v (get h b 3) < pow2 52 /\ v (get h b 4) < pow2 52
+let lemma_prime_limb_size () = assert_norm (pow2 (5 * 51) > pow2 255 - 19)
 
-let reduced_before_mul_l h b =
-  let _ = 0 in
-  live h b /\ v (get h b 0) < pow2 53 /\ v (get h b 1) < pow2 53 /\ v (get h b 2) < pow2 53
-  /\ v (get h b 3) < pow2 53 /\ v (get h b 4) < pow2 53
+open Hacl.UInt64
 
-let reduced_before_mul_r h b =
-  let _ = 0 in
-  live h b /\ v (get h b 0) < pow2 54 /\ v (get h b 1) < pow2 54 /\ v (get h b 2) < pow2 54
-  /\ v (get h b 3) < pow2 54 /\ v (get h b 4) < pow2 54
+inline_for_extraction let v x = v x
 
-let reduced_wide h b =
-  let _ = 0 in
-  live h b /\ w (get h b 0) < pow2 52 /\ w (get h b 1) < pow2 52 /\ w (get h b 2) < pow2 52
-  /\ w (get h b 3) < pow2 52 /\ w (get h b 4) < pow2 52
+inline_for_extraction let limb_zero = uint64_to_sint64 0uL
+inline_for_extraction let limb_one  = uint64_to_sint64 1uL
 
-let reducible h b =
-  (* TODO *)
-  admit()
+(* Addition primitives *)
+inline_for_extraction let limb_add a b = add a b
+inline_for_extraction let limb_add_mod a b = add_mod a b
+(* Subtraction primitives *)
+inline_for_extraction let limb_sub a b = sub a b
+inline_for_extraction let limb_sub_mod a b = sub_mod a b
+(* Multiplication primitives *)
+inline_for_extraction let limb_mul a b = mul a b
+inline_for_extraction let limb_mul_mod a b = mul_mod a b
+
+(* Bitwise operators *)
+inline_for_extraction let limb_logand a b = logand a b
+inline_for_extraction let limb_logxor a b = logxor a b
+inline_for_extraction let limb_logor  a b = logor  a b
+inline_for_extraction let limb_lognot a   = lognot a
+
+(* Shift operators *)
+inline_for_extraction let limb_shift_right a s = shift_right a s
+inline_for_extraction let limb_shift_left  a s = shift_left a s
+
+inline_for_extraction let limb_eq_mask a b  = eq_mask a b
+inline_for_extraction let limb_gte_mask a b = gte_mask a b
+inline_for_extraction let limb_gt_mask a b  = gt_mask a b
+inline_for_extraction let limb_lt_mask a b  = lt_mask a b
+inline_for_extraction let limb_lte_mask a b = lte_mask a b
+
+inline_for_extraction let limb_to_byte x = assert_norm(pow2 8 = 256); sint64_to_sint8 x
+inline_for_extraction let byte_to_limb x = sint8_to_sint64 x
+
+open Hacl.UInt128
+
+inline_for_extraction let w x = Hacl.UInt128.v x
+
+inline_for_extraction let wide_zero = sint64_to_sint128 (uint64_to_sint64 0uL)
+inline_for_extraction let wide_one  = sint64_to_sint128 (uint64_to_sint64 1uL)
+
+(* Addition primitives *)
+inline_for_extraction let wide_add a b = add a b
+inline_for_extraction let wide_add_mod a b = add_mod a b
+(* Subtraction primitives *)
+inline_for_extraction let wide_sub a b = sub a b
+inline_for_extraction let wide_sub_mod a b = sub_mod a b
+(* Multiplication primitives *)
+inline_for_extraction let wide_mul a b = mul a b
+inline_for_extraction let wide_mul_mod a b = mul_mod a b
+
+(* Bitwise operators *)
+inline_for_extraction let wide_logand a b = logand a b
+inline_for_extraction let wide_logxor a b = logxor a b
+inline_for_extraction let wide_logor  a b = logor  a b
+inline_for_extraction let wide_lognot a   = lognot a
+
+(* Shift operators *)
+inline_for_extraction let wide_shift_right a s = shift_right a s
+inline_for_extraction let wide_shift_left  a s = shift_left a s
+
+inline_for_extraction let wide_eq_mask a b  = eq_mask a b
+inline_for_extraction let wide_gte_mask a b = gte_mask a b
+inline_for_extraction let wide_gt_mask a b  = gt_mask a b
+inline_for_extraction let wide_lt_mask a b  = lt_mask a b
+inline_for_extraction let wide_lte_mask a b = lte_mask a b
+
+inline_for_extraction let mul_wide x y = mul_wide x y
+
+inline_for_extraction let limb_to_wide x = sint64_to_sint128 x
+inline_for_extraction let wide_to_limb x = sint128_to_sint64 x
+
+(* let reduced_after_mul h b = *)
+(*   let _ = 0 in *)
+(*   live h b /\ v (get h b 0) < pow2 52 /\ v (get h b 1) < pow2 52 /\ v (get h b 2) < pow2 52 *)
+(*   /\ v (get h b 3) < pow2 52 /\ v (get h b 4) < pow2 52 *)
+
+(* let reduced_before_mul_l h b = *)
+(*   let _ = 0 in *)
+(*   live h b /\ v (get h b 0) < pow2 53 /\ v (get h b 1) < pow2 53 /\ v (get h b 2) < pow2 53 *)
+(*   /\ v (get h b 3) < pow2 53 /\ v (get h b 4) < pow2 53 *)
+
+(* let reduced_before_mul_r h b = *)
+(*   let _ = 0 in *)
+(*   live h b /\ v (get h b 0) < pow2 54 /\ v (get h b 1) < pow2 54 /\ v (get h b 2) < pow2 54 *)
+(*   /\ v (get h b 3) < pow2 54 /\ v (get h b 4) < pow2 54 *)
+
+(* let reduced_wide h b = *)
+(*   let _ = 0 in *)
+(*   live h b /\ w (get h b 0) < pow2 52 /\ w (get h b 1) < pow2 52 /\ w (get h b 2) < pow2 52 *)
+(*   /\ w (get h b 3) < pow2 52 /\ w (get h b 4) < pow2 52 *)
+
+(* let reducible h b = *)
+(*   (\* TODO *\) *)
+(*   admit() *)
