crypto/bignum/Hacl.Bignum.Modulo.fsti
@@ -12,23 +12,31 @@ open Hacl.Bignum.Limb
 
 module U32 = FStar.UInt32
 
-
-val shift_reduce:
-  b:felem ->
-  i:ctr{U32.v i < len} ->
-  Stack unit
-    (requires (fun h -> live h b /\ reduced h b))
-    (ensures (fun h0 _ h1 -> live h0 b /\ reduced h1 b /\ modifies_1 b h0 h1 /\ live h1 b
-      /\ eval h1 b % prime = eval h0 b * (template (U32.v i)) % prime))
+(** Pure definition of the "add_zero" function **)
+val added_zero: mem -> felem -> mem -> felem -> Type0
 
 val add_zero:
   b:felem ->
   Stack unit
-    (requires (fun h -> live h b /\ reduced h b))
+    (requires (fun h -> live h b /\ reduced_after_mul h b))
     (ensures (fun h0 _ h1 -> live h0 b /\ live h1 b /\ modifies_1 b h0 h1
       /\ eval h1 b % prime = eval h0 b % prime
+      /\ added_zero h1 b h0 b
       (* TODO: more fine grained condition or do an extra reduction step *)
     ))
+
+
+val reduced_after_sr: mem -> felem -> Type0
+val shift_reduced: mem -> felem -> mem -> felem -> Type0
+
+
+val shift_reduce:
+  b:felem ->
+  Stack unit
+    (requires (fun h -> live h b /\ reduced_after_mul h b))
+    (ensures (fun h0 _ h1 -> live h0 b /\ reduced_after_sr h1 b /\ modifies_1 b h0 h1 /\ live h1 b
+      /\ eval h1 b % prime = (eval h0 b * pow2 limb_size) % prime))
+
 
 val carry_top:
   b:felem ->
@@ -36,11 +44,13 @@ val carry_top:
   (requires (fun _ -> true))
   (ensures (fun _ _ _ -> true))
 
+
 val reduce:
   b:felem ->
   Stack unit
   (requires (fun h -> true))
   (ensures (fun _ _ _ -> true))
+
 
 val reduce_wide:
   b:felem_wide ->
