crypto/bignum/Hacl.Bignum.Predicates.fsti
@@ -1,0 +1,12 @@
+module Hacl.Bignum.Predicates
+
+
+(** Predicate associated to 'workable' bigintegers, restored after each bigint computation **)
+val reduced_after_mul: h:mem -> b:felem -> GTot Type0
+val reduced_before_mul_l: h:mem -> b:felem -> GTot Type0
+val reduced_before_mul_r: h:mem -> b:felem -> GTot Type0
+val reduced_wide: h:mem -> b:felem_wide -> GTot Type0
+
+(** Predicate associated to 'workable' bigintegers, restored after each bigint computation **)
+val reducible: h:mem -> b:felem -> GTot Type0
+
